examples/new_stack/NewStack23Aproof.v
@@ -247,7 +247,7 @@ Section SIMMODSEM.
           }
           rewrite add_disj_insert; ss. eapply sim_fresh_k; et.
         }
-      - unfold KModSem.transl_fun_tgt, new_body. rewrite X. cbn. steps. post_call.
+      - unfold KModSem.transl_fun, new_body. rewrite X. cbn. steps. post_call.
         rename x into h. force_l. exists h. steps. rewrite Any.upcast_downcast. steps.
         assert(S:=SIM h). rewrite _GUARANTEE in *. inv S; ss. force_l; ss. steps.
 
@@ -258,7 +258,7 @@ Section SIMMODSEM.
     econs; ss.
     { unfold NewStack2.pop_body, cfun, cfun2. init. harg. post_call.
       destruct x; destruct (Any.split varg_src) eqn:X; des_ifs_safe; mDesAll; ss; des; subst.
-      - unfold KModSem.transl_fun_tgt. steps.
+      - unfold KModSem.transl_fun. steps.
         rewrite Any.upcast_split. cbn. steps. rewrite Any.upcast_downcast in *. clarify. steps.
         rewrite Any.upcast_downcast in *. clarify. steps. renamer. rename n into h. rename a into stk0.
 
@@ -315,7 +315,7 @@ Section SIMMODSEM.
     econs; ss.
     { unfold NewStack2.push_body, cfun, cfun2. init. harg. post_call.
       destruct x; destruct (Any.split varg_src) eqn:X; des_ifs_safe; mDesAll; ss; des; subst.
-      - unfold KModSem.transl_fun_tgt. steps.
+      - unfold KModSem.transl_fun. steps.
         rewrite Any.upcast_split. cbn. steps. rewrite Any.upcast_downcast in *. clarify. steps.
         rewrite Any.upcast_downcast in *. clarify. renamer. steps.
         rename n into h. rename l into stk0. rename v into x.
